\documentclass{article}
\usepackage{amsmath,amssymb,kotex,multicol, enumitem}


\title{곱셈공식}
\date{\today}
\author{}

\begin{document}

%\begin{enumerate}[label=(\alph*)]
%\item
%\end{enumerate}

\begin{align*}
\text{곱셈공식}\\
(1) &\quad(a+b)^2 = a^2+2ab+b^2\\
(2) &\quad(a-b)^2 = a^2-2ab+b^2\\
(3) &\quad(a+b)(a-b) = a^2-b^2\\[10pt]
(4) &\quad(a+b)^3 = a^3+3a^2b+3ab^2+b^3\\
(5) &\quad(a-b)^3 = a^3-3a^2b+3ab^2-b^3\\[10pt]
(6) &\quad(a+b)(a^2-ab+b^2) = a^3-b^3\\
(7) &\quad(a-b)(a^2+ab+b^2) = a^3+b^3\\[10pt]
(8) &\quad(a+b+c)^2 = a^2+b^2+c^2+2(ab+bc+ca)\\
(9) &\quad(a+b+c)(a^2+b^2+c^2-ab-bc-ca) = a^3+b^3+c^3-3abc\\[10pt]
(10) &\quad(a+b)^3 = a^3+b^3+3ab(a+b)\\
(11) &\quad(a-b)^3 = a^3-b^3-3ab(a-b)\\[10pt]
(12) &\quad(x-a)(x-b)=x^2-(a+b)x+ab\\
(13) &\quad(x-a)(x-b)(x-c)=x^3-(a+b+c)x^2+(ab+bc+ca)x-abc\\[10pt]
(14) &\quad(a^2+ab+b^2)(a^2-ab+b^2)=a^4+a^2b^2+b^4\\
\end{align*}


\end{document}