\documentclass[a4paper,twocolumn]{oblivoir}
\usepackage{amsmath,amssymb,amsthm,kotex,graphicx}
\usepackage{fapapersize}
\usefapapersize{210mm,297mm,10mm,*,10mm,*}
\newcounter{num}
\newcommand{\defi}[1]
{\bigskip\noindent\refstepcounter{num}\textbf{정의 \arabic{num}) #1}\par\noindent}
\newcommand{\theo}[1]
{\bigskip\noindent\refstepcounter{num}\textbf{정리 \arabic{num}) #1}\par\noindent}
\newcommand{\exam}[1]
{\bigskip\noindent\refstepcounter{num}\textbf{예시 \arabic{num}) #1}\par\noindent}
\newcommand{\prob}[1]
{\bigskip\noindent\refstepcounter{num}\textbf{문제 \arabic{num}) #1}\par\noindent}
\newcommand{\proo}
{\bigskip\textsf{증명)}\par}

\title{수지 : 함수의 극한 복습}
\date{\today}
\author{}
%%%%
\begin{document}
\maketitle

%
\exam{\(y=x^2-4\)}
{\centering\includegraphics[width=0.4\textwidth]{55}}
\begin{gather*}
\lim_{x\to1}(x^2-4)=\\
\lim_{x\to0}(x^2-4)=\\
\lim_{x\to\infty}(x^2-4)=\\
\lim_{x\to-\infty}(x^2-4)=
\end{gather*}
\newpage

%
\prob{\(y=-x^2+4\)}
{\centering\includegraphics[width=0.4\textwidth]{55}}
\begin{gather*}
\lim_{x\to1}(-x^2+4)=\\
\lim_{x\to2}(-x^2+4)=\\
\lim_{x\to\infty}(-x^2+4)=\\
\lim_{x\to-\infty}(-x^2+4)=
\end{gather*}
\newpage

%
\exam{\(y=\sqrt x\)}
{\centering\includegraphics[width=0.4\textwidth]{55}}
\begin{gather*}
\lim_{x\to4}\sqrt x=\\
\lim_{x\to3}\sqrt x=\\
\lim_{x\to\infty}\sqrt x=
\end{gather*}

%
\prob{\(y=-\sqrt x\)}
{\centering\includegraphics[width=0.4\textwidth]{55}}
\begin{gather*}
\lim_{x\to1}(-\sqrt x)=\\
\lim_{x\to3}(-\sqrt x)=\\
\lim_{x\to\infty}(-\sqrt x)=
\end{gather*}
\newpage

%
\exam{\(y=\frac{2x+1}{x-1}\)}
{\centering\includegraphics[width=0.4\textwidth]{55}}
\begin{gather*}
\lim_{x\to2}\frac{2x+1}{x-1}=\\
\lim_{x\to\infty}\frac{2x+1}{x-1}=\\
\lim_{x\to-\infty}\frac{2x+1}{x-1}=\\
\lim_{x\to1+}\frac{2x+1}{x-1}=\\
\lim_{x\to1-}\frac{2x+1}{x-1}=
\end{gather*}

%
\prob{\(y=\frac{2x-3}{x-2}\)}
{\centering\includegraphics[width=0.4\textwidth]{55}}
\begin{gather*}
\lim_{x\to1}\frac{2x-3}{x-2}=\\
\lim_{x\to\infty}\frac{2x-3}{x-2}=\\
\lim_{x\to-\infty}\frac{2x-3}{x-2}=\\
\lim_{x\to2+}\frac{2x-3}{x-2}=\\
\lim_{x\to2-}\frac{2x-3}{x-2}=
\end{gather*}
\newpage

%
\exam{\(y=[x]\)}
{\centering\includegraphics[width=0.4\textwidth]{55}}
\begin{gather*}
\lim_{x\to\frac32}[x]=\\
\lim_{x\to1+}[x]=\\
\lim_{x\to1-}[x]=\\
\lim_{x\to-1+}[x]=\\
\lim_{x\to-1-}[x]=
\end{gather*}

%
\prob{\(y=x-[x]\)}
{\centering\includegraphics[width=0.4\textwidth]{55}}
\begin{gather*}
\lim_{x\to\frac32}(x-[x])=\\
\lim_{x\to1+}(x-[x])=\\
\lim_{x\to1-}(x-[x])=\\
\lim_{x\to-1+}(x-[x])=\\
\lim_{x\to-1-}(x-[x])=
\end{gather*}
\newpage

%
\exam{\(y=|x-2|\)}
{\centering\includegraphics[width=0.4\textwidth]{55}}
\begin{gather*}
\lim_{x\to1}|x-2|=\\
\lim_{x\to2}|x-2|=\\
\lim_{x\to3}|x-2|=\\
\lim_{x\to\infty}|x-2|=\\
\lim_{x\to-\infty}|x-2|=
\end{gather*}

%
\prob{\(y=|2x+2|\)}
{\centering\includegraphics[width=0.4\textwidth]{55}}
\begin{gather*}
\lim_{x\to-1}|2x+2|=\\
\lim_{x\to2}|2x+2|=\\
\lim_{x\to\infty}|2x+2|=\\
\lim_{x\to-\infty}|2x+2|=
\end{gather*}
\newpage

%
\exam{\(y=\frac{x-2}{|x-2|}\)}
{\centering\includegraphics[width=0.4\textwidth]{55}}
\begin{gather*}
\lim_{x\to1}\frac{x-2}{|x-2|}=\\
\lim_{x\to3}\frac{x-2}{|x-2|}=\\
\lim_{x\to2+}\frac{x-2}{|x-2|}=\\
\lim_{x\to2-}\frac{x-2}{|x-2|}=
\end{gather*}

%
\prob{\(y=\frac x{|x|}\)}
{\centering\includegraphics[width=0.4\textwidth]{55}}
\begin{gather*}
\lim_{x\to-2}\frac x{|x|}=\\
\lim_{x\to3}\frac x{|x|}=\\
\lim_{x\to0+}\frac x{|x|}=\\
\lim_{x\to0-}\frac x{|x|}=
\end{gather*}
\newpage

%
\exam{\(y=\frac{x^2+x-2}{x-1}\)}
{\centering\includegraphics[width=0.4\textwidth]{55}}
\begin{gather*}
\lim_{x\to0}\frac{x^2+x-2}{x-1}=\\
\lim_{x\to2}\frac{x^2+x-2}{x-1}=\\
\lim_{x\to1+}\frac{x^2+x-2}{x-1}=\\
\lim_{x\to1-}\frac{x^2+x-2}{x-1}=
\end{gather*}

%
\prob{\(y=\frac{x^2-3x+2}{x-2}\)}
{\centering\includegraphics[width=0.4\textwidth]{55}}
\begin{gather*}
\lim_{x\to1}\frac{x^2-3x+2}{x-2}=\\
\lim_{x\to3}\frac{x^2-3x+2}{x-2}=\\
\lim_{x\to2+}\frac{x^2-3x+2}{x-2}=\\
\lim_{x\to2-}\frac{x^2-3x+2}{x-2}=
\end{gather*}

\end{document}